Hashmap/Benchmark/FilterMap.lean
@@ -1,0 +1,184 @@
+import Hashmap.DHashMap.Basic
+
+/-!
+Example run below. This benchmark tests three different implementations of the `filterMap` operation.
+
+* `filterMap₁` filters the buckets using a non-tail-recursive filterMap operation on AssocLists and computes the
+  size of the resulting map afterwards
+* `filterMap₂` is lifted from Batteries and computes the size of the resulting map while performing the mapping
+  using a tail-recursive function `AssocList α β → ULift Nat → AssocList α γ × ULift Nat`.
+* `filterMap₃` is like `filterMap₁`, but tail-recursive.
+
+As the sample data below shows, `filterMap₂` is about 40% slower than the other two implementations.
+The reason for this is most likely that `filterMap₂` performs an additional `Prod.mk` constructor call
+per bucket (recall that hash maps have a lot of buckets). It might be possible to fix this by somehow
+convincing the compiler to reuse the memory from the current iteration in the next iteration, but it's
+not clear how one would need to change the code to make this work.
+
+-/
+
+open MyLean
+
+def lowercase : List Char :=
+  ['a', 'b', 'c', 'd', 'e', 'f', 'g', 'h', 'i', 'j', 'k', 'l', 'm',
+   'n', 'o', 'p', 'q', 'r', 's', 't', 'u', 'v', 'w', 'x', 'y', 'z']
+
+partial def mkStrings (len num : Nat) : Array String := Id.run do
+  if len = 0 then
+    return #[""]
+
+  let inner := mkStrings (len - 1) ((num + 25) / 26)
+  let mut hv : Nat := 0
+  let mut ans : Array String := #[]
+  for i in inner do
+    for c in lowercase do
+      ans := ans.push (i.push c)
+      hv := hv + 1
+      if hv = num then
+        break
+    if hv = num then
+      break
+  ans
+
+@[noinline] def mkMyStrings (num len : Nat) : IO (Array String) := do
+  return mkStrings num len
+
+def sz : Nat := 2000000
+
+/-- Percentage of mappings that survive the filtering process. The small this number,
+    the more pronounced the difference between the implementations is. -/
+def resultSize : Nat := 5
+
+---------------------------
+-- Option 1: proper hash function
+@[noinline] def growInsert (strings : Array String) : IO (DHashMap String (fun _ => Nat)) := do
+  let mut m : DHashMap String (fun _ => Nat) := DHashMap.empty sz
+  let mut i := 0
+  for s in strings do
+    m := m.insert s i
+    i := i + 1
+  return m
+---------------------------
+-- Option 2: bad hash function (with insert changed to insertUnsafe because otherwise inserting takes way too long)
+-- instance : Hashable String where
+--   hash _ := 1
+-- @[noinline] def growInsert (strings : Array String) : IO (DHashMap String (fun _ => Nat)) := do
+--   let mut m : DHashMap String (fun _ => Nat) := DHashMap.empty sz
+--   let mut i := 0
+--   for s in strings do
+--     m := m.insertUnsafe s i
+--     i := i + 1
+--   return m
+---------------------------
+
+@[noinline] def performFilterMap₁ : DHashMap String (fun _ => Nat) → IO Nat :=
+  fun m => pure (m.filterMap₁ (fun _ v => if v % 100 < resultSize then some (v + 1) else none)).size
+
+@[noinline] def performFilterMap₂ : DHashMap String (fun _ => Nat) → IO Nat :=
+  fun m => pure (m.filterMap₂ (fun _ v => if v % 100 < resultSize then some (v + 1) else none)).size
+
+@[noinline] def performFilterMap₃ : DHashMap String (fun _ => Nat) → IO Nat :=
+  fun m => pure (m.filterMap₃ (fun _ v => if v % 100 < resultSize then some (v + 1) else none)).size
+
+@[noinline] def performBenchmark₁ (strings : Array String) : IO Unit := do
+  let m ← growInsert strings
+  let _ ← timeit "filterMap₁" $ performFilterMap₁ m
+
+@[noinline] def performBenchmark₂ (strings : Array String) : IO Unit := do
+  let m ← growInsert strings
+  let _ ← timeit "filterMap₂" $ performFilterMap₂ m
+
+@[noinline] def performBenchmark₃ (strings : Array String) : IO Unit := do
+  let m ← growInsert strings
+  let _ ← timeit "filterMap₃" $ performFilterMap₃ m
+
+def histogram {α : Type u} {β : α → Type v} [BEq α] [Hashable α]
+    (m : DHashMap α β) : DHashMap Nat (fun _ => Nat) := Id.run do
+  let mut hist : DHashMap Nat (fun _ => Nat) := ∅
+  for bucketSize in m.1.buckets.map AssocList.length do
+    let newCount : Nat := match hist.findConst? bucketSize with
+      | none => 1
+      | some n => n + 1
+    hist := hist.insert bucketSize newCount
+  hist
+
+def main (_ : List String) : IO UInt32 := do
+  let strings ← mkMyStrings 8 sz
+  let hist := DHashMap.toListModel ((histogram (← growInsert strings)).1.buckets)
+  IO.println hist
+  for _ in [:20] do
+    performBenchmark₁ strings
+  for _ in [:20] do
+    performBenchmark₂ strings
+  for _ in [:20] do
+    performBenchmark₃ strings
+  return 0
+
+
+/-!
+
+```
+[⟨0, 2603848⟩, ⟨1, 1241048⟩, ⟨2, 296138⟩, ⟨3, 47044⟩, ⟨4, 5639⟩, ⟨5, 537⟩, ⟨6, 47⟩, ⟨7, 3⟩]
+filterMap₁ 279ms
+filterMap₁ 277ms
+filterMap₁ 278ms
+filterMap₁ 279ms
+filterMap₁ 280ms
+filterMap₁ 295ms
+filterMap₁ 278ms
+filterMap₁ 277ms
+filterMap₁ 279ms
+filterMap₁ 279ms
+filterMap₁ 279ms
+filterMap₁ 279ms
+filterMap₁ 278ms
+filterMap₁ 279ms
+filterMap₁ 279ms
+filterMap₁ 275ms
+filterMap₁ 277ms
+filterMap₁ 276ms
+filterMap₁ 277ms
+filterMap₁ 276ms
+filterMap₂ 407ms
+filterMap₂ 408ms
+filterMap₂ 409ms
+filterMap₂ 409ms
+filterMap₂ 406ms
+filterMap₂ 405ms
+filterMap₂ 406ms
+filterMap₂ 408ms
+filterMap₂ 409ms
+filterMap₂ 406ms
+filterMap₂ 408ms
+filterMap₂ 407ms
+filterMap₂ 409ms
+filterMap₂ 395ms
+filterMap₂ 392ms
+filterMap₂ 390ms
+filterMap₂ 392ms
+filterMap₂ 393ms
+filterMap₂ 390ms
+filterMap₂ 388ms
+filterMap₃ 261ms
+filterMap₃ 259ms
+filterMap₃ 260ms
+filterMap₃ 263ms
+filterMap₃ 264ms
+filterMap₃ 263ms
+filterMap₃ 267ms
+filterMap₃ 260ms
+filterMap₃ 260ms
+filterMap₃ 261ms
+filterMap₃ 259ms
+filterMap₃ 290ms
+filterMap₃ 277ms
+filterMap₃ 279ms
+filterMap₃ 277ms
+filterMap₃ 278ms
+filterMap₃ 278ms
+filterMap₃ 277ms
+filterMap₃ 278ms
+filterMap₃ 277ms
+```
+
+-/
