Hashmap/Benchmark/Insert.lean
@@ -1,0 +1,153 @@
+import Batteries.Data.HashMap
+import Hashmap.DHashMap.Basic
+
+/-!
+Example run below. This benchmark tests the `insert` operation of the present hash map, the Lean hash map
+and the Batteries hash map.
+
+Takeaways:
+* The Batteries hash map is about 10% slower, due to https://github.com/leanprover/lean4/issues/4191
+* Implementing `mkIdx` in C++ doesn't seem to make a difference, which isn't too surprising since all
+  of the operations happen on USize, which should be fast when compiled from Lean. The two versions
+  probably only differ slightly in their initial boxing/unboxing, but I didn't check this in detail.
+
+-/
+
+open MyLean
+
+def lowercase : List Char :=
+  [ 'a', 'b', 'c', 'd', 'e', 'f', 'g', 'h', 'i', 'j', 'k', 'l', 'm',
+    'n', 'o', 'p', 'q', 'r', 's', 't', 'u', 'v', 'w', 'x', 'y', 'z']
+
+partial def mkStrings (len num : Nat) : Array String := Id.run do
+  if len = 0 then
+    return #[""]
+
+  let inner := mkStrings (len - 1) ((num + 25) / 26)
+  let mut hv : Nat := 0
+  let mut ans : Array String := #[]
+  for i in inner do
+    for c in lowercase do
+      ans := ans.push (i.push c)
+      hv := hv + 1
+      if hv = num then
+        break
+    if hv = num then
+      break
+  ans
+
+@[noinline] def mkMyStrings (num len : Nat) : IO (Array String) := do
+  return mkStrings num len
+
+def sz : Nat := 3000000
+def presize : Bool := false
+
+@[noinline] def growInsert' (strings : Array String) : (DHashMap String (fun _ => Nat)) := Id.run do
+  let mut m : DHashMap String (fun _ => Nat) := bif presize then DHashMap.empty sz else DHashMap.empty
+  let mut i := 0
+  for s in strings do
+    m := m.insert s i
+    i := i + 1
+  return m
+
+@[noinline] def growInsert'' (a : Array String) : IO (DHashMap String (fun _ => Nat)) := do
+  return growInsert' a
+
+@[noinline] def growInsertL (strings : Array String) : (Lean.HashMap String Nat) := Id.run do
+  let mut m : Lean.HashMap String Nat := bif presize then Lean.mkHashMap sz else Lean.mkHashMap
+  let mut i := 0
+  for s in strings do
+    m := m.insert s i
+    i := i + 1
+  return m
+
+@[noinline] def growInsertL' (strings : Array String) : IO (Lean.HashMap String Nat) := do
+  return growInsertL strings
+
+@[noinline] def growInsertB (strings : Array String) : (Batteries.HashMap String Nat) := Id.run do
+  let mut m : Batteries.HashMap String Nat := bif presize then Batteries.mkHashMap sz else Batteries.mkHashMap
+  let mut i := 0
+  for s in strings do
+    m := m.insert s i
+    i := i + 1
+  return m
+
+@[noinline] def growInsertB' (strings : Array String) : IO (Batteries.HashMap String Nat) := do
+  return growInsertB strings
+
+def main (_ : List String) : IO UInt32 := do
+  let strings ← timeit "mkMyStrings" $ mkMyStrings 8 sz
+  for _ in [:20] do
+    let _ ← timeit "This hash map" $ growInsert'' strings
+  for _ in [:20] do
+    let _ ← timeit "Lean hash map" $ growInsertL' strings
+  for _ in [:20] do
+    let _ ← timeit "Bats hash map" $ growInsertB' strings
+  return 0
+
+/-!
+```
+mkMyStrings 136ms
+This hash map 918ms
+This hash map 895ms
+This hash map 947ms
+This hash map 859ms
+This hash map 934ms
+This hash map 889ms
+This hash map 896ms
+This hash map 890ms
+This hash map 896ms
+This hash map 893ms
+This hash map 892ms
+This hash map 894ms
+This hash map 899ms
+This hash map 898ms
+This hash map 894ms
+This hash map 951ms
+This hash map 902ms
+This hash map 897ms
+This hash map 897ms
+This hash map 899ms
+Lean hash map 895ms
+Lean hash map 886ms
+Lean hash map 895ms
+Lean hash map 885ms
+Lean hash map 915ms
+Lean hash map 896ms
+Lean hash map 896ms
+Lean hash map 902ms
+Lean hash map 899ms
+Lean hash map 889ms
+Lean hash map 896ms
+Lean hash map 897ms
+Lean hash map 888ms
+Lean hash map 894ms
+Lean hash map 897ms
+Lean hash map 893ms
+Lean hash map 905ms
+Lean hash map 899ms
+Lean hash map 897ms
+Lean hash map 896ms
+Bats hash map 1.03s
+Bats hash map 1.04s
+Bats hash map 1.03s
+Bats hash map 1.03s
+Bats hash map 1.04s
+Bats hash map 1.04s
+Bats hash map 1.03s
+Bats hash map 1.04s
+Bats hash map 1.03s
+Bats hash map 1.03s
+Bats hash map 1.03s
+Bats hash map 1.03s
+Bats hash map 1.03s
+Bats hash map 1.03s
+Bats hash map 1.04s
+Bats hash map 1.03s
+Bats hash map 1.02s
+Bats hash map 1.02s
+Bats hash map 1.03s
+Bats hash map 1.03s
+```
+
+-/
